generational/spec/GC.Gen.CheneyGraphReadiness.fst
@@ -37,6 +37,7 @@ module ChunkedMajorGC = GC.Spec.ChunkedMajorGC.Defs
 module ChunkedMajorGCRoots = GC.Spec.ChunkedMajorGC.Roots
 module ChunkedMajorGCCorr = GC.Spec.ChunkedMajorGC.Correctness
 module ChunkedMajorGCGraph = GC.Spec.ChunkedMajorGC.Graph
+module ChunkedMarkTargetMembership = GC.Spec.ChunkedMarkBounded.TargetMembership
 
 #push-options "--split_queries always --z3rlimit 1 --fuel 0 --ifuel 0"
 private let aligned_gt_ge_plus_mword (x z: nat)
@@ -3709,6 +3710,83 @@ let chunked_cheney_collect_then_major_gc_live_subgraph_from_static_raw_target_po
   GenMajorGCBridge.chunked_major_gc_bounded_after_gray_roots_raw_target_policy_from_static
     collect.cmc_major major_roots cap mark_fuel;
   chunked_cheney_collect_then_major_gc_live_subgraph_from_raw_target_policy
+    minor major fp roots alloc_fuel fresh major_roots cap mark_fuel
+
+let chunked_cheney_collect_then_major_gc_live_subgraph_from_pre_gray_static_raw_target_policy
+  (minor: minor_state) (major: MH.major_heap) (fp: U64.t)
+  (roots: seq U64.t) (alloc_fuel: nat) (fresh: MH.heap_chunk)
+  (major_roots: seq obj_addr)
+  (cap: nat{cap > 0})
+  (mark_fuel: nat)
+  : Lemma
+    (requires
+      minor_wf minor /\
+      alloc_fuel > 1 /\
+      GenInv.chunked_collection_heap_shape minor major fp alloc_fuel /\
+      SpecMajorAlloc.major_fl_chain_terminates major fp alloc_fuel = true /\
+      GenInv.chunked_chain_objects_blue major fp alloc_fuel /\
+      chunked_minor_preflight_value_policy minor major fp roots fresh /\
+      (let r =
+       SpecMajorAlloc.ensure_major_head_capacity_spec
+        major fp alloc_fuel
+        (PromotionDemand.minor_promotion_demand minor + 1)
+        fresh in
+       let collect =
+       ChunkedCheney.chunked_cheney_collect_spec
+        minor r.capacity_major_out r.capacity_fp_out roots
+        r.capacity_fuel_out in
+       GenInv.chunked_collection_heap_shape
+        collect.cmc_minor collect.cmc_major collect.cmc_fp
+        r.capacity_fuel_out /\
+       GenMajorGCBridge.chunked_major_roots_nonblue
+        collect.cmc_major major_roots /\
+       GenMajorGCBridge.chunked_major_edge_gen_field_witness
+        collect.cmc_major /\
+       GenMajorGCBridge.chunked_major_field_targets_non_infix
+        collect.cmc_major /\
+       ChunkedMarkTargetMembership.chunked_scanned_raw_targets_in_major
+        collect.cmc_major /\
+       Seq.length (MH.major_objects collect.cmc_major) <= cap /\
+       mark_fuel > 0 /\
+       mark_fuel >= Seq.length (MH.major_objects collect.cmc_major)))
+    (ensures
+      chunked_cheney_collect_after_minor_promotion_head_preflight_post
+       minor major fp roots alloc_fuel fresh /\
+      (let r =
+       SpecMajorAlloc.ensure_major_head_capacity_spec
+        major fp alloc_fuel
+        (PromotionDemand.minor_promotion_demand minor + 1)
+        fresh in
+       let collect =
+       ChunkedCheney.chunked_cheney_collect_spec
+        minor r.capacity_major_out r.capacity_fp_out roots
+        r.capacity_fuel_out in
+       let (major_final, fp_final) =
+       ChunkedMajorGC.chunked_major_gc_bounded
+        (ChunkedMajorGCRoots.chunked_gray_roots
+          collect.cmc_major major_roots)
+        cap mark_fuel in
+       ChunkedMajorGCGraph.chunked_major_live_subgraph_preserved
+        collect.cmc_major major_final
+        (ChunkedMajorGCCorr.chunked_major_initial_reachable_live
+         collect.cmc_major major_roots)))
+  =
+  let r =
+    SpecMajorAlloc.ensure_major_head_capacity_spec
+      major fp alloc_fuel
+      (PromotionDemand.minor_promotion_demand minor + 1)
+      fresh in
+  let collect =
+    ChunkedCheney.chunked_cheney_collect_spec
+      minor r.capacity_major_out r.capacity_fp_out roots
+      r.capacity_fuel_out in
+  GenInv.chunked_collection_heap_shape_elim
+    collect.cmc_minor collect.cmc_major collect.cmc_fp r.capacity_fuel_out;
+  GenInv.chunked_major_alloc_shape_elim
+    collect.cmc_major collect.cmc_fp r.capacity_fuel_out;
+  GenMajorGCBridge.chunked_major_gc_bounded_after_gray_roots_static_raw_target_policy_from_pre_gray
+    collect.cmc_major major_roots cap mark_fuel;
+  chunked_cheney_collect_then_major_gc_live_subgraph_from_static_raw_target_policy
     minor major fp roots alloc_fuel fresh major_roots cap mark_fuel
 #pop-options
 
